cleanups on level_polys & level_points_view

crypto_examples/mulntt_ct/mulntt_ct_rec.dfy
@@ -13,14 +13,22 @@ module mulntt_ct_rec {
 
     import opened nth_root
     import opened ntt_index
-    // function method A(): seq<elem>
-    //     ensures |A()| == N == pow2(LOGN).full;
+
+    function method A(): seq<elem>
+        ensures |A()| == N == pow2(LOGN).full;
 
     function method block_count(m: pow2_t): nat
         requires 0 <= m.exp <= LOGN;
     {
         pow2_div(pow2(LOGN), m).full
     }
+
+    // lemma block_count_product_lemma(m: pow2_t)
+    //     requires 0 <= m.exp <= LOGN;
+    //     ensures block_count(m) * m.full == N;
+    // {
+    //     Nth_root_lemma();
+    // }
 
     lemma block_count_half_lemma(m: pow2_t)
         requires 1 <= m.exp <= LOGN;
@@ -45,78 +53,118 @@ module mulntt_ct_rec {
         LemmaMulEqualityConverse(half, left.full, right.full * 2);
     }
 
-    datatype lpolys = lpolys_cons(blocks: seq<seq<elem>>, bsize: pow2_t)
+    type n_sized = s: seq<elem>
+        | |s| == N == pow2(LOGN).full witness *
+    
+    lemma point_view_index_bound_lemma(i: nat, j: nat, bsize: pow2_t)
+        requires bsize.exp <= LOGN;
+        requires i < block_count(bsize);
+        requires j < bsize.full;
+        ensures 0 <= i + j * block_count(bsize) < N;
     {
-        predicate level_wf()
-        {
-            && unifromly_sized(blocks, bsize)
-            && 0 <= bsize.exp <= LOGN
-            && block_count(bsize) == |blocks|
+        var count := block_count(bsize);
+        calc {
+            i + j * count;
+            <=
+            count - 1 + j * count;
+            <= { LemmaMulInequality(j, bsize.full - 1, count); }
+            count - 1 + (bsize.full - 1) * count;
+            { LemmaMulIsDistributive(count, bsize.full, 1); }
+            count - 1 + bsize.full * count - count;
+            bsize.full * count - 1;
+            { Nth_root_lemma(); }
+            N - 1;
         }
 
-        function method {:opaque} build_smaller_level(): (lps: lpolys)
-            requires level_wf();
-            requires 1 <= bsize.exp <= LOGN;
-            ensures lps.level_wf();
-            ensures lps.bsize == pow2_half(bsize);
-            ensures |lps.blocks| == 2 * |blocks|;
-        {
-            reveal unifromly_sized();
-            pow2_basics(bsize);
-            block_count_half_lemma(bsize);
-            var new_size := pow2_half(bsize);
-            var new_count := |blocks| * 2;
-            var new_blocks := seq(new_count, n requires 0 <= n < new_count => 
-                if n % 2 == 0 then even_indexed_items(blocks[n/2], bsize)
-                else odd_indexed_items(blocks[n/2], bsize));
-            lpolys_cons(new_blocks, new_size)
-        }
-
-        // lemma base_level_correct()
-        //     requires blocks == [A()];
-        //     requires bsize.exp == LOGN;
-        //     ensures level_wf();
-        // {
-        //     reveal level_wf();
-        //     Nth_root_lemma();
-        //     assert bsize.full == N;
-        // }
-
-        lemma level_index_correspondence_lemma(i: nat, sl: lpolys)
-            requires level_wf();
-            requires 1 <= bsize.exp <= LOGN;
-            requires sl == build_smaller_level();
-            requires i < |blocks|;
-            ensures |blocks[i]| == bsize.full;
-            ensures 2 * i + 1 < |sl.blocks|;
-            ensures even_indexed_items(blocks[i], bsize) == sl.blocks[2 * i];
-            ensures |sl.blocks[2 * i]| == pow2_half(bsize).full;
-            ensures odd_indexed_items(blocks[i], bsize) == sl.blocks[2 * i + 1];
-            ensures |sl.blocks[2 * i + 1]| == pow2_half(bsize).full;
-        {
-            reveal unifromly_sized();
-            reveal build_smaller_level();
-        }
+        LemmaMulStrictlyPositiveAuto();
     }
 
-    // function method build_lpolys(bsize: pow2_t): (lps: lpolys)
-    //     requires bsize.exp <= LOGN;
-    //     ensures lps.level_wf();
-    //     ensures lps.bsize == bsize;
-    //     decreases LOGN - bsize.exp;
-    // {
-    //     if bsize.exp == LOGN then
-    //         var l := lpolys_cons([A()], bsize);
-    //         l.base_level_correct();
-    //         l
-    //     else
-    //         var prev := build_lpolys(pow2_double(bsize));
-    //         // assert 1 <= pow2_double(bsize).exp <= LOGN;
-    //         prev.build_smaller_level()
-    // }
+    function point_view_index(i: nat, j: nat, bsize: pow2_t): (offset: nat)
+        requires bsize.exp <= LOGN;
+        requires i < block_count(bsize);
+        requires j < bsize.full;
+        ensures offset < N;
+    {
+        point_view_index_bound_lemma(i, j, bsize);
+        i + j * block_count(bsize)
+    }
 
-    // function method build_all_lpolys(): seq<lpolys>
-    // {
+    function points_view(a: n_sized, i: nat, bsize: pow2_t): (v: seq<elem>)
+        requires bsize.exp <= LOGN;
+        requires i < block_count(bsize);
+        // ensures |v| == bsize.full;
+    {
+        var size := bsize.full;
+        seq(size, j requires 0 <= j < size => a[point_view_index(i, j, bsize)])
+    }
 
-    // }
+    // interpret an n_sized buffer as a level view
+    // contains blocks of points, each block has bsize
+    function level_points_view(a: n_sized, bsize: pow2_t): (vs: seq<seq<elem>>)
+        requires bsize.exp <= LOGN;
+        ensures unifromly_sized(vs, bsize);
+    {
+        var count := block_count(bsize);
+        var vs := seq(count, i requires 0 <= i < count => points_view(a, i, bsize));
+        assert unifromly_sized(vs, bsize) by {
+            reveal unifromly_sized();
+        }
+        vs
+    }
+
+    function method {:opaque} build_lower_level(higher: seq<seq<elem>>, bsize: pow2_t): (lower: seq<seq<elem>>)
+        requires 1 <= bsize.exp <= LOGN;
+        requires unifromly_sized(higher, bsize);
+        ensures unifromly_sized(lower, pow2_half(bsize));
+    {
+        reveal unifromly_sized();
+        pow2_basics(bsize);
+        block_count_half_lemma(bsize);
+        var new_size := pow2_half(bsize);
+        var new_count := |higher| * 2;
+        seq(new_count, n requires 0 <= n < new_count => 
+            if n % 2 == 0 then even_indexed_items(higher[n/2], bsize)
+            else odd_indexed_items(higher[n/2], bsize))
+    }
+
+    lemma base_level_correct()
+        ensures unifromly_sized([A()], pow2(LOGN));
+    {
+        reveal unifromly_sized();
+    }
+
+    // construct polys level view 
+    // each block is a poly, has bsize coefficients
+    function level_polys(bsize: pow2_t): (lps: seq<seq<elem>>)
+        requires 1 <= bsize.exp <= LOGN;
+        decreases LOGN - bsize.exp;
+        ensures unifromly_sized(lps, bsize);
+    {
+        if bsize.exp == LOGN then
+            base_level_correct();
+            [A()]
+        else
+            assert 1 <= bsize.exp <= LOGN;
+            var double_size := pow2_double(bsize);
+            assert 1 <= double_size.exp <= LOGN;
+            var higher := level_polys(double_size);
+            build_lower_level(higher, double_size)
+    }
+
+    lemma level_polys_index_correspondence_lemma(
+        higher: seq<seq<elem>>, hi_size: pow2_t, i: nat, 
+        lower: seq<seq<elem>>)
+        requires 1 <= hi_size.exp <= LOGN;
+        requires i < |higher|;
+        requires unifromly_sized(higher, hi_size);
+        requires build_lower_level(higher, hi_size) == lower;
+        ensures |higher[i]| == hi_size.full;
+        ensures 2 * i + 1 < |lower|;
+        ensures even_indexed_items(higher[i], hi_size) == lower[2 * i];
+        ensures odd_indexed_items(higher[i], hi_size) == lower[2 * i + 1];
+        ensures |lower[2 * i]| == |lower[2 * i + 1]| == pow2_half(hi_size).full;
+    {
+        reveal unifromly_sized();
+        reveal build_lower_level();
+    }
 }
